DeBruijnSn/Looping.lean
@@ -74,7 +74,7 @@ inductive SN : Term → Type where
 | normLambda : SN t → SN (.lam t)
 | normNE : NE t → SN t
 | normVarApp : SN (.app t (.var n)) → SN t
-| normWH : WeakHeadExp t t' u → SN t' → SN u → SN t
+| normWH : WeakHeadExp t t' u → SN u → SN t' → SN t
 inductive NE : Term → Type where
 | varNE : NE (.var n)
 | appNE : NE n → SN t → NE (.app n t)
@@ -96,17 +96,31 @@ inductive TypeTerm : Ctx → Term → Ty → Type where
 | unfoldTy : ∀ Γ t, Γ ⊢ t :+ .d → Γ ⊢ t :+ .d ⇒ .d
 | foldTy : ∀ Γ t, Γ ⊢ t :+ .d ⇒ .d → Γ ⊢ t :+ .d
 
+
+
+axiom D : Term → Type
+
+axiom neD : ∀ ne : Term, NE ne → D ne
+axiom snD : ∀ t : Term, D t → SN t
+axiom whD : ∀ t t' u : Term,
+  WeakHeadExp t t' u → SN u → D t' → D t
+
+axiom neSN : ∀ (t : Term) (p : NE t) , snD t (neD t p) = .normNE p
+axiom whSN : ∀ (t t' u : Term) (p : WeakHeadExp t t' u) (sn_u : SN u) (base_t' : D t'),
+  snD t (whD t t' u p sn_u base_t') = .normWH p sn_u (snD t' base_t')
+
+
 -- This axiom is false, of course. But it'll allow us to prove normalization
 -- in an interesting way.
-axiom foldType t : (∀ u, SN u → SN (.app t u)) → SN t
+axiom foldType t : (∀ u, D u → D (.app t u)) → D t
 -- This one is true but whatever
-axiom unfoldType t : SN t → (∀ u, SN u → SN (.app t u))
+axiom unfoldType t : D t → (∀ u, D u → D (.app t u))
 
 notation "⟦" ty "⟧" => (interpTy ty)
 
 @[simp]
 def interpTy : Ty → Term → Type
-| .d => SN
+| .d => D
 | ty₁ ⇒ ty₂ => λ t ↦ ∀ u, ⟦ty₁⟧ u → ⟦ty₂⟧ (.app t u)
 
 def validSubst (Γ : Ctx) (σ : Subst) := ∀ n A, Γ.get? n = .some A → ⟦A⟧ (σ n)
@@ -267,7 +281,7 @@ theorem wh_comp : WeakHeadExp t t' u → SN u → ⟦A⟧ t' → ⟦A⟧ t :=
 by
   cases A <;> simp
   case d =>
-    intros wh sn_u sn_t'; apply SN.normWH (u := u) <;> trivial
+    intros wh sn_u sn_t'; apply whD <;> trivial
   case arrow A₁ A₂ =>
     intros wh sn_u comp_t' u' comp_u'
     apply wh_comp; apply WeakHeadExp.appWH; trivial
@@ -280,7 +294,7 @@ mutual
 theorem sn_comp : ⟦A⟧ t → SN t :=
 by
   cases A <;> simp
-  case d => intros; trivial
+  case d => intros; apply snD; trivial
   case arrow =>
     intro comp_t
     apply SN.normVarApp
@@ -291,7 +305,7 @@ by
 theorem neutral_comp : NE n → ⟦A⟧ n :=
 by
   cases A <;> simp
-  case d => intro ne_n; constructor; trivial
+  case d => intro ne_n; apply neD; trivial
   case arrow =>
     intros neutral_n u comp_u
     have norm_u := sn_comp comp_u
@@ -299,7 +313,7 @@ by
     constructor <;> trivial
 end
 
-theorem soundness (d : Γ ⊢ t :+ A) (valid : Γ ⊧ σ): ⟦A⟧ (t⟨σ⟩) :=
+theorem soundness (d : Γ ⊢ t :+ A) (valid : Γ ⊧ σ) : ⟦A⟧ (t⟨σ⟩) :=
 by
   cases d <;> simp [subst]
   case varTy n h => apply valid; trivial
@@ -327,12 +341,12 @@ by
     apply unfoldType;
     apply (soundness ih); trivial
     trivial
-  case foldTy =>
+  case foldTy ty_t =>
     apply foldType; intros
-    have ihT : ⟦Ty.d ⇒ Ty.d⟧ (t⟨σ⟩) := by apply soundness <;> trivial
+    have ihT := soundness ty_t valid
     simp at ihT; apply ihT; trivial
-  termination_by soundness d valid => d
 
+#print soundness
 
 theorem idS_valid : Γ ⊧ idS :=
 by
@@ -369,7 +383,8 @@ by
     constructor
     case a =>
       constructor
-      case a => apply TypeTerm.unfoldTy; apply TypeTerm.varTy; simp [List.get?]; rfl
+      case a => apply TypeTerm.unfoldTy; apply TypeTerm.varTy; simp [List.get?]
       case a => apply TypeTerm.varTy; simp [List.get?]
 
+#print sn_Omega
 -- #reduce sn_Omega
