Main.lean
@@ -1,4 +1,6 @@
 import «DeBruijnSn»
 
+def hello : String := "world"
+
 def main : IO Unit :=
   IO.println s!"Hello, {hello}!"
